AP/Sokoban/MovableBoxConjecture/Defs.lean
@@ -1,3 +1,9 @@
 import AP.Sokoban.Card
 
 namespace Sokoban
+
+def State.AlwaysMovable (s : State) : Prop :=
+  sys.WF s ∧ ∀ s₁, sys.Reachable s s₁ → ∃ s₂, sys.Reachable s₁ s₂ ∧ s₁.boxes ≠ s₂.boxes
+
+def MovableBoxConjecture : Prop :=
+  ∃ (s : State), s.AlwaysMovable
