AP/Sokoban/MovableBoxConjecture/Basic.lean
@@ -1,3 +1,26 @@
 import AP.Sokoban.MovableBoxConjecture.Defs
 
 namespace Sokoban
+
+open State
+
+variable {s s₁ s₂ s₃ : State}
+
+theorem State.AlwaysMovable.wf (h : s.AlwaysMovable) : sys.WF s := h.1
+
+theorem boxes_ne_empty_of_alwaysMovable (h : s.AlwaysMovable) : s.boxes ≠ ∅ := by
+  rcases h with ⟨h₁, h₂⟩
+  specialize h₂ s (by rfl)
+  choose s₁ h₂ h₃ using h₂
+  contrapose! h₃
+  symm; simp [h₃]
+  rw [←Set'.size_eq_zero_iff] at h₃ ⊢; rw [←h₃]
+  exact State.size_boxes_eq_of_reachable h₂
+
+theorem alwaysMovable_iff_alt₁ : s.AlwaysMovable ↔ sys.WF s ∧ s.boxes ≠ ∅ ∧
+∀ s₁, sys.Reachable s s₁ → ∃ s₂, sys.Reachable s₁ s₂ ∧ s₁.boxes ≠ s₂.boxes := by
+  constructor
+  · intro h
+    use h.wf, boxes_ne_empty_of_alwaysMovable h, h.2
+  · rintro ⟨h₁, h₂, h₃⟩
+    exact ⟨h₁, h₃⟩
